To prove the equality of $\mu_b \gamma_b = \mu_b \gamma_b \mu_b \gamma_b$, it's easier to prove the inequalities $\mu_b \gamma_b \leq \mu_b \gamma_b \mu_b \gamma_b$ and $\mu_b \gamma_b > \mu_b \gamma_b \mu_b \gamma_b$.

First, let's prove $\mu_b \gamma_b \leq \mu_b \gamma_b \mu_b \gamma_b$. Let $\gamma_b$ be idempotent, then starting from the identity $\mu_b \gamma_b = \mu_b \gamma_b$ the following equality holds:

$\mu_b \gamma_b \gamma_b \gamma_b = \mu_b \gamma_b$

$\implies$ $\mu_b \gamma_b \mu_b \gamma_b \geq \mu_b \gamma_b$ (1)

Second, let's prove $\mu_b \gamma_b > \mu_b \gamma_b \mu_b \gamma_b$. Let $\mu_b$ be idempotent, then starting from the identity $\mu_b \gamma_b = \mu_b \gamma_b$ the following equality holds:

$\mu_b \mu_b \mu_b \gamma_b = \mu_b \gamma_b$

$\implies$ $\mu_b \gamma_b \mu_b \gamma_b < \mu_b \gamma_b$ (2)

From (1) and (2) it is proven that $\mu_b \gamma_b = \mu_b \gamma_b \mu_b \gamma_b$